src/Spec/Equiv.v
@@ -1,8 +1,9 @@
-Require Import ConcurExec.
+Require Import Spec.ConcurExec.
+Require Import Spec.ThreadsState.
+Require Import Spec.BasicEquiv.
 Require Import Relations.Relation_Operators.
 Require Import Morphisms.
 Require Import ProofAutomation.
-Require Import Spec.ThreadsState.
 Require Import Helpers.Instances.
 Require Import List.
 Require Import Omega.
@@ -20,16 +21,6 @@ Section OpSemantics.
 
   Local Obligation Tactic := try RelInstance_t.
 
-  (** A strong notion of execution equivalence, independent of semantics *)
-
-  Definition exec_equiv_ts (ts1 ts2 : threads_state Op) :=
-    forall (s : State) tr,
-      exec op_step s ts1 tr <->
-      exec op_step s ts2 tr.
-
-  Global Program Instance exec_equiv_ts_equivalence :
-    Equivalence exec_equiv_ts.
-
   (** A stronger notion of equivalence where number of steps taken must be
     identical *)
 
@@ -38,7 +29,7 @@ Section OpSemantics.
       exec_till op_step n s ts1 tr <->
       exec_till op_step n s ts2 tr.
 
-  Local Definition exec_equiv_N n T (p1 p2: proc Op T) :=
+  Definition exec_equiv_N n T (p1 p2: proc Op T) :=
     forall ts tid, exec_equiv_ts_N n (ts [[tid := Proc p1]]) (ts [[tid := Proc p2]]).
 
   (** A strong notion of equivalence for programs inside atomic sections.
@@ -57,48 +48,6 @@ Section OpSemantics.
     Proper (atomic_equiv ==> atomic_equiv ==> iff) (@atomic_equiv T).
   Proof.
     typeclasses eauto.
-  Qed.
-
-  Local Definition exec_equiv_opt (p1 : maybe_proc Op) p2 :=
-    forall (ts : threads_state _) tid,
-      exec_equiv_ts (ts [[ tid := p1 ]]) (ts [[ tid := p2 ]]).
-
-  Definition exec_equiv `(p1 : proc Op T) (p2 : proc _ T) :=
-    exec_equiv_opt (Proc p1) (Proc p2).
-
-  Definition exec_equiv_rx `(p1 : proc Op T) (p2 : proc _ T) :=
-    forall TR (rx : T -> proc _ TR),
-      exec_equiv (Bind p1 rx) (Bind p2 rx).
-
-  Global Program Instance exec_equiv_opt_equivalence :
-    Equivalence exec_equiv_opt.
-
-  Global Program Instance exec_equiv_equivalence :
-    Equivalence (@exec_equiv T).
-
-  Global Program Instance exec_equiv_rx_equivalence :
-    Equivalence (@exec_equiv_rx T).
-
-  Global Instance thread_upd_exec_equiv_proper :
-    Proper (eq ==> eq ==> exec_equiv_opt ==> exec_equiv_ts) (@thread_upd Op).
-  Proof.
-    intros.
-    intros ts0 ts1 H; subst.
-    intros tid tid' H'; subst.
-    intros o0 o1 H'.
-
-    unfold exec_equiv_ts; split; intros.
-    - apply H'; eauto.
-    - apply H'; eauto.
-  Qed.
-
-  Global Instance Proc_exec_equiv_proper :
-    Proper (exec_equiv ==> exec_equiv_opt) (@Proc Op T).
-  Proof.
-    intros.
-    unfold exec_equiv.
-    intros ts0 ts1 H; subst.
-    eauto.
   Qed.
 
   (** Trace inclusion for an entire threads_state *)
@@ -124,7 +73,7 @@ Section OpSemantics.
   Qed.
 
   Global Instance exec_equiv_ts_to_trace_incl_ts :
-    subrelation exec_equiv_ts trace_incl_ts.
+    subrelation (exec_equiv_ts op_step) trace_incl_ts.
   Proof.
     unfold subrelation; intros.
     unfold trace_incl_ts; intros.
@@ -309,209 +258,6 @@ numbers of steps *)
     thread_upd_ind' p;
     [ solve_ExecEquiv | .. ].
 
-  Local Notation exec_p p := (exec_tid _ _ _ p _ _ _ _) (only parsing).
-
-  Theorem exec_equiv_ret_None : forall `(v : T),
-      exec_equiv_opt (Proc (Ret v)) NoProc.
-  Proof.
-    split; intros.
-    - ExecEquiv.
-    - change tr with (prepend tid nil tr).
-      eapply ExecOne with (tid := tid).
-      autorewrite with t; eauto.
-      rewrite mapping_finite; auto.
-      econstructor.
-      match goal with
-      | |- context[S (thread_max ?ts)] =>
-        rewrite thread_upd_same_eq with (tid := S (thread_max ts))
-      end.
-      autorewrite with t; eauto.
-      rewrite mapping_finite; eauto.
-  Qed.
-
-  (* TODO: define trace_incl between two n's for all ts and continuations, prove
-     this for as many things as possible.
-
-   Then prove generic theorems that prove the others are special cases. *)
-
-  (* trace_incl_rx' is the right definition; steps should not be used unless
-     needed, really only hold for monad associativity *)
-
-  Theorem exec_equiv_bind_ret : forall `(p : proc Op T),
-      exec_equiv (Bind p Ret) p.
-  Proof.
-    unfold exec_equiv; split; intros.
-
-    - ExecEquiv' p.
-      destruct result0.
-      + ExecPrefix tid tid'.
-        eapply exec_equiv_ret_None; eauto.
-      + ExecPrefix tid tid'.
-
-    - ExecEquiv' p.
-      destruct result; guess_ExecPrefix.
-      eapply exec_equiv_ret_None; eauto.
-  Qed.
-
-  Global Instance exec_equiv_rx_to_exec_equiv :
-    subrelation (@exec_equiv_rx T) exec_equiv.
-  Proof.
-    unfold subrelation, exec_equiv_rx; intros.
-    rewrite <- exec_equiv_bind_ret with (p := x).
-    rewrite <- exec_equiv_bind_ret with (p := y).
-    eauto.
-  Qed.
-
-  Local Theorem exec_equiv_rx_proof_helper : forall `(p1 : proc Op T) p2,
-      (forall tid tid' `(s : State) s' (ts: threads_state _) tr spawned evs `(rx : _ -> proc _ TR) result,
-          exec_tid op_step tid s (Bind p1 rx) s' result spawned evs ->
-          ts tid' = NoProc ->
-          tid <> tid' ->
-          exec op_step s' (ts [[tid' := spawned]] [[tid := match result with
-                                                           | inl _ => NoProc
-                                                           | inr p' => Proc p'
-                                                           end]]) tr ->
-          exec op_step s (ts [[tid := Proc (Bind p2 rx)]]) (prepend tid evs tr)) ->
-      (forall tid tid' `(s : State) s' (ts: threads_state _) tr evs spawned `(rx : _ -> proc _ TR) result,
-          exec_tid op_step tid s (Bind p2 rx) s' result spawned evs ->
-          ts tid' = NoProc ->
-          tid <> tid' ->
-          exec op_step s' (ts [[tid' := spawned]] [[tid := match result with
-                                                           | inl _ => NoProc
-                                                           | inr p' => Proc p'
-                                                           end]]) tr ->
-          exec op_step s (ts [[tid := Proc (Bind p1 rx)]]) (prepend tid evs tr)) ->
-      exec_equiv_rx p1 p2.
-  Proof.
-    split; intros.
-    - ExecEquiv.
-    - ExecEquiv.
-  Qed.
-
-  Theorem exec_equiv_ret_bind : forall `(v : T) `(p : T -> proc Op T'),
-      exec_equiv_rx (Bind (Ret v) p) (p v).
-  Proof.
-    intros.
-    eapply exec_equiv_rx_proof_helper; intros; exec_tid_simpl.
-    - simpl.
-      rewrite thread_upd_same_eq with (tid:=tid') in H2 by eauto.
-      eauto.
-    - rewrite <- app_nil_l with (l := evs).
-      rewrite prepend_app.
-      ExecPrefix tid tid'.
-      ExecPrefix tid tid'.
-  Qed.
-
-  Theorem exec_equiv_atomicret_ret : forall `(v : T),
-      exec_equiv_rx (Atomic (Ret v)) (Ret v).
-  Proof.
-    intros.
-    eapply exec_equiv_rx_proof_helper; intros; exec_tid_simpl.
-    - repeat atomic_exec_inv.
-      ExecPrefix tid tid'.
-    - ExecPrefix tid tid'.
-  Qed.
-
-  Theorem exec_equiv_bind_bind : forall `(p1 : proc Op T1) `(p2 : T1 -> proc Op T2) `(p3 : T2 -> proc Op T3),
-      exec_equiv_rx (Bind (Bind p1 p2) p3) (Bind p1 (fun v => Bind (p2 v) p3)).
-  Proof.
-    split; intros.
-    - ExecEquiv' p1.
-      ExecPrefix tid tid'.
-      destruct result0; eauto.
-    - ExecEquiv' p1.
-      ExecPrefix tid tid'.
-      destruct result; eauto.
-  Qed.
-
-  Theorem exec_equiv_bind_a : forall `(p : proc Op T) `(p1 : T -> proc _ T') p2,
-      (forall x, exec_equiv (p1 x) (p2 x)) ->
-      exec_equiv (Bind p p1) (Bind p p2).
-  Proof.
-    unfold exec_equiv; split; intros.
-    - ExecEquiv' p.
-      ExecPrefix tid tid'.
-      destruct result0; eauto.
-      eapply H; eauto.
-
-    - ExecEquiv' p.
-      ExecPrefix tid tid'.
-      destruct result0; eauto.
-      eapply H; eauto.
-  Qed.
-
-  Theorem exec_equiv_until : forall `(p : option T -> proc Op T) (c : T -> bool) v,
-      exec_equiv_rx (Until c p v) (until1 c p v).
-  Proof.
-    intros.
-    eapply exec_equiv_rx_proof_helper; intros.
-    - exec_tid_simpl.
-      rewrite thread_upd_same_eq with (tid:=tid') in H2 by congruence.
-      simpl; eauto.
-    - rewrite <- app_nil_l with (l := evs).
-      rewrite prepend_app.
-      ExecPrefix tid tid'.
-      ExecPrefix tid tid'.
-  Qed.
-
-  Theorem exec_equiv_spawn : forall `(p1 : proc Op T) p2,
-      exec_equiv p1 p2 ->
-      exec_equiv_rx (Spawn p1) (Spawn p2).
-  Proof.
-    intros.
-    eapply exec_equiv_rx_proof_helper; intros.
-    - exec_tid_simpl.
-      ExecPrefix tid tid'.
-      rewrite thread_upd_ne_comm in * by auto.
-      match goal with
-      | H : exec_equiv _ _ |- _ =>
-        apply H; eauto
-      end.
-    - exec_tid_simpl.
-      ExecPrefix tid tid'.
-      rewrite thread_upd_ne_comm in * by auto.
-      match goal with
-      | H : exec_equiv _ _ |- _ =>
-        apply H; eauto
-      end.
-  Qed.
-
-  Local Theorem exec_equiv_congruence : forall T (p1 p2: proc Op T) T' (rx1 rx2: T -> proc Op T'),
-      exec_equiv_rx p1 p2 ->
-      (forall x, exec_equiv_rx (rx1 x) (rx2 x)) ->
-      exec_equiv_rx (Bind p1 rx1) (Bind p2 rx2).
-  Proof.
-    intros.
-    unfold exec_equiv_rx; intros.
-    repeat rewrite exec_equiv_bind_bind.
-    etransitivity.
-    eapply H.
-    eapply exec_equiv_bind_a; intros.
-    eapply H0.
-  Qed.
-
-  Global Instance Bind_exec_equiv_proper :
-    Proper (exec_equiv_rx ==>
-                          pointwise_relation T exec_equiv_rx ==>
-                          @exec_equiv_rx TR) Bind.
-  Proof.
-    unfold Proper, respectful, pointwise_relation; intros.
-    apply exec_equiv_congruence; auto.
-  Qed.
-
-  Global Instance Spawn_exec_equiv_proper :
-    Proper (@exec_equiv T ==> exec_equiv_rx) Spawn.
-  Proof.
-    unfold Proper, respectful, pointwise_relation; intros.
-    apply exec_equiv_spawn; auto.
-  Qed.
-
-  Global Instance exec_proper_exec_equiv :
-    Proper (eq ==> exec_equiv_ts ==> eq ==> iff) (@exec Op State op_step).
-  Proof.
-    unfold Proper, respectful; intros; subst; eauto.
-  Qed.
-
   Local Theorem exec_equiv_N_bind_bind : forall `(p1 : proc Op T1) `(p2 : T1 -> proc Op T2) `(p3 : T2 -> proc Op T3) n,
       exec_equiv_N n (Bind (Bind p1 p2) p3) (Bind p1 (fun v => Bind (p2 v) p3)).
   Proof.
@@ -589,7 +335,7 @@ numbers of steps *)
   Qed.
 
   Global Instance Atomic_proper_atomic_equiv :
-    Proper (atomic_equiv ==> @exec_equiv_rx T) Atomic.
+    Proper (atomic_equiv ==> exec_equiv_rx op_step (T:=T)) Atomic.
   Proof.
     intros.
     intros p1 p2 H.
@@ -623,7 +369,7 @@ numbers of steps *)
     PreOrder (@trace_incl T).
 
   Global Instance exec_equiv_to_trace_incl :
-    subrelation (@exec_equiv T) (@trace_incl T).
+    subrelation (exec_equiv op_step (T:=T)) (@trace_incl T).
   Proof.
     unfold subrelation; intros.
     unfold trace_incl, trace_incl_ts, trace_incl_ts_s; intros.
@@ -683,7 +429,7 @@ numbers of steps *)
   Qed.
 
   Global Instance trace_incl_s_exec_equiv_proper :
-    Proper (exec_equiv ==> exec_equiv ==> iff)
+    Proper (exec_equiv op_step ==> exec_equiv op_step ==> iff)
            (@trace_incl_s s tid T).
   Proof.
     intros.
@@ -703,7 +449,7 @@ numbers of steps *)
   Qed.
 
   Global Instance trace_incl_exec_equiv_proper :
-    Proper (exec_equiv ==> exec_equiv ==> iff)
+    Proper (exec_equiv op_step ==> exec_equiv op_step ==> iff)
            (@trace_incl T).
   Proof.
     unfold Proper, respectful, trace_incl; intros.
@@ -1035,6 +781,7 @@ numbers of steps *)
     end.
   Qed.
 
+
   Local Theorem trace_incl_rx_until_helper :
     forall T (p1 p2 : option T -> proc Op T)
       (c : T -> bool) n v,
@@ -1136,8 +883,8 @@ numbers of steps *)
   (** Reuse the complicated proof about [Until]. *)
 
   Theorem exec_equiv_until_body : forall `(p1 : option T -> proc Op T) p2 c v,
-      (forall a, exec_equiv_rx (p1 a) (p2 a)) ->
-      exec_equiv_rx (Until c p1 v) (Until c p2 v).
+      (forall a, exec_equiv_rx op_step (p1 a) (p2 a)) ->
+      exec_equiv_rx op_step (Until c p1 v) (Until c p2 v).
   Proof.
     split; intros.
     - eapply exec_to_counter in H0; deex.
@@ -1155,9 +902,9 @@ numbers of steps *)
 
   Global Instance Until_exec_equiv_proper :
     Proper (eq ==>
-               pointwise_relation _ exec_equiv_rx ==>
+               pointwise_relation _ (exec_equiv_rx op_step) ==>
                eq ==>
-               @exec_equiv_rx T) Until.
+               exec_equiv_rx op_step (T:=T)) Until.
   Proof.
     unfold Proper, respectful, pointwise_relation; intros; subst.
     apply exec_equiv_until_body; eauto.
