src/Spec/BasicEquiv.v
@@ -1,0 +1,349 @@
+Require Import Spec.ConcurExec.
+Require Import Spec.ThreadsState.
+
+Require Import ProofAutomation.
+Require Import Helpers.Instances.
+Require Import Morphisms.
+
+Section OpSemantics.
+
+  Context {Op:Type -> Type}.
+  Context {State:Type}.
+  Variable op_step: OpSemantics Op State.
+
+  Local Obligation Tactic := try RelInstance_t.
+
+  (** A strong notion of execution equivalence, independent of semantics *)
+
+  Definition exec_equiv_ts (ts1 ts2 : threads_state Op) :=
+    forall (s : State) tr,
+      exec op_step s ts1 tr <->
+      exec op_step s ts2 tr.
+
+  Global Program Instance exec_equiv_ts_equivalence :
+    Equivalence exec_equiv_ts.
+
+  Local Definition exec_equiv_opt (p1 : maybe_proc Op) p2 :=
+    forall (ts : threads_state _) tid,
+      exec_equiv_ts (ts [[ tid := p1 ]]) (ts [[ tid := p2 ]]).
+
+  Definition exec_equiv `(p1 : proc Op T) (p2 : proc _ T) :=
+    exec_equiv_opt (Proc p1) (Proc p2).
+
+  Definition exec_equiv_rx `(p1 : proc Op T) (p2 : proc _ T) :=
+    forall TR (rx : T -> proc _ TR),
+      exec_equiv (Bind p1 rx) (Bind p2 rx).
+
+  Global Program Instance exec_equiv_opt_equivalence :
+    Equivalence exec_equiv_opt.
+
+  Global Program Instance exec_equiv_equivalence :
+    Equivalence (@exec_equiv T).
+
+  Global Program Instance exec_equiv_rx_equivalence :
+    Equivalence (@exec_equiv_rx T).
+
+  Global Instance thread_upd_exec_equiv_proper :
+    Proper (eq ==> eq ==> exec_equiv_opt ==> exec_equiv_ts) (@thread_upd Op).
+  Proof.
+    intros.
+    intros ts0 ts1 H; subst.
+    intros tid tid' H'; subst.
+    intros o0 o1 H'.
+
+    unfold exec_equiv_ts; split; intros.
+    - apply H'; eauto.
+    - apply H'; eauto.
+  Qed.
+
+  Global Instance Proc_exec_equiv_proper :
+    Proper (exec_equiv ==> exec_equiv_opt) (@Proc Op T).
+  Proof.
+    intros.
+    unfold exec_equiv.
+    intros ts0 ts1 H; subst.
+    eauto.
+  Qed.
+
+  Hint Constructors exec_tid.
+  Hint Constructors exec_till.
+
+  Hint Extern 1 (exec _ _ _ _ _) =>
+  match goal with
+  | |- exec_till _ _ _ ?ts _ => first [ is_evar ts; fail 1 | eapply ConcurExec.exec_ts_eq ]
+  end : exec.
+
+  Ltac thread_upd_ind p :=
+    let ind H := induction H; intros; subst; eauto; NoProc_upd in
+    match goal with
+    | H : exec _ _ (thread_upd ?ts ?tid (Proc ?pp)) _ |- _ =>
+      remember (thread_upd ts tid (Proc pp));
+      generalize dependent ts;
+      generalize dependent p;
+      ind H
+    | H : exec_till _ _ _ (thread_upd ?ts ?tid (Proc ?pp)) _ |- _ =>
+      remember (thread_upd ts tid (Proc pp));
+      generalize dependent ts;
+      generalize dependent p;
+      ind H
+    end.
+
+  Ltac guess_ExecPrefix :=
+    match goal with
+    | [ H: thread_get _ ?tid' = NoProc |- context[prepend ?tid _ _] ] =>
+      ExecPrefix tid tid'
+    end.
+
+  Ltac solve_ExecEquiv :=
+    match goal with
+    | [ H: context[thread_get (thread_upd _ ?tid _) ?tid'] |- _ ] =>
+      cmp_ts tid' tid; repeat maybe_proc_inv;
+      exec_tid_simpl;
+      remove_redundant_upds;
+      try (solve [ eauto ] ||
+           solve [ guess_ExecPrefix ])
+    end.
+
+  Ltac ExecEquiv p :=
+    thread_upd_ind p;
+    [ solve_ExecEquiv | .. ].
+
+  Theorem exec_equiv_ret_None : forall `(v : T),
+      exec_equiv_opt (Proc (Ret v)) NoProc.
+  Proof.
+    split; intros.
+    - ExecEquiv tt.
+    - change tr with (prepend tid nil tr).
+      eapply ExecOne with (tid := tid).
+      autorewrite with t; eauto.
+      rewrite mapping_finite; auto.
+      econstructor.
+      match goal with
+      | |- context[S (thread_max ?ts)] =>
+        rewrite thread_upd_same_eq with (tid := S (thread_max ts))
+      end.
+      autorewrite with t; eauto.
+      rewrite mapping_finite; eauto.
+  Qed.
+
+  Theorem exec_equiv_rx_proof_helper : forall `(p1 : proc Op T) p2,
+      (forall tid tid' `(s : State) s' (ts: threads_state _) tr spawned evs `(rx : _ -> proc _ TR) result,
+          exec_tid op_step tid s (Bind p1 rx) s' result spawned evs ->
+          ts tid' = NoProc ->
+          tid <> tid' ->
+          exec op_step s' (ts [[tid' := spawned]] [[tid := match result with
+                                                           | inl _ => NoProc
+                                                           | inr p' => Proc p'
+                                                           end]]) tr ->
+          exec op_step s (ts [[tid := Proc (Bind p2 rx)]]) (prepend tid evs tr)) ->
+      (forall tid tid' `(s : State) s' (ts: threads_state _) tr evs spawned `(rx : _ -> proc _ TR) result,
+          exec_tid op_step tid s (Bind p2 rx) s' result spawned evs ->
+          ts tid' = NoProc ->
+          tid <> tid' ->
+          exec op_step s' (ts [[tid' := spawned]] [[tid := match result with
+                                                           | inl _ => NoProc
+                                                           | inr p' => Proc p'
+                                                           end]]) tr ->
+          exec op_step s (ts [[tid := Proc (Bind p1 rx)]]) (prepend tid evs tr)) ->
+      exec_equiv_rx p1 p2.
+  Proof.
+    split; intros.
+    - ExecEquiv tt.
+    - ExecEquiv tt.
+  Qed.
+
+  Theorem exec_equiv_rx_bind_bind : forall `(p1 : proc Op T1) `(p2 : T1 -> proc Op T2) `(p3 : T2 -> proc Op T3),
+      exec_equiv_rx (Bind (Bind p1 p2) p3) (Bind p1 (fun v => Bind (p2 v) p3)).
+  Proof.
+    split; intros.
+    - ExecEquiv p1.
+      ExecPrefix tid tid'.
+      destruct result0; eauto.
+    - ExecEquiv p1.
+      ExecPrefix tid tid'.
+      destruct result; eauto.
+  Qed.
+
+  Theorem exec_equiv_ret_bind : forall `(v : T) `(p : T -> proc Op T'),
+      exec_equiv_rx (Bind (Ret v) p) (p v).
+  Proof.
+    intros.
+    eapply exec_equiv_rx_proof_helper; intros; exec_tid_simpl.
+    - simpl.
+      rewrite thread_upd_same_eq with (tid:=tid') in H2 by eauto.
+      eauto.
+    - abstract_tr.
+      ExecPrefix tid tid'.
+      ExecPrefix tid tid'.
+      rewrite <- prepend_app; simpl; auto.
+  Qed.
+
+  Theorem exec_equiv_bind_ret : forall `(p : proc Op T),
+      exec_equiv (Bind p Ret) p.
+  Proof.
+    unfold exec_equiv; split; intros.
+
+    - ExecEquiv p.
+      destruct result0.
+      + ExecPrefix tid tid'.
+        eapply exec_equiv_ret_None; eauto.
+      + ExecPrefix tid tid'.
+
+    - ExecEquiv p.
+      destruct result; guess_ExecPrefix.
+      eapply exec_equiv_ret_None; eauto.
+  Qed.
+
+  Global Instance exec_equiv_rx_to_exec_equiv :
+    subrelation (@exec_equiv_rx T) exec_equiv.
+  Proof.
+    unfold subrelation, exec_equiv_rx; intros.
+    rewrite <- exec_equiv_bind_ret with (p := x).
+    rewrite <- exec_equiv_bind_ret with (p := y).
+    eauto.
+  Qed.
+
+  Theorem exec_equiv_bind_bind : forall `(p1 : proc Op T1) `(p2 : T1 -> proc Op T2) `(p3 : T2 -> proc Op T3),
+      exec_equiv (Bind (Bind p1 p2) p3) (Bind p1 (fun v => Bind (p2 v) p3)).
+  Proof.
+    intros.
+    rewrite exec_equiv_rx_bind_bind; reflexivity.
+  Qed.
+
+  Theorem exec_equiv_bind_a : forall `(p : proc Op T) `(p1 : T -> proc _ T') p2,
+      (forall x, exec_equiv (p1 x) (p2 x)) ->
+      exec_equiv (Bind p p1) (Bind p p2).
+  Proof.
+    unfold exec_equiv; split; intros.
+    - ExecEquiv p.
+      ExecPrefix tid tid'.
+      destruct result0; eauto.
+      eapply H; eauto.
+
+    - ExecEquiv p.
+      ExecPrefix tid tid'.
+      destruct result0; eauto.
+      eapply H; eauto.
+  Qed.
+
+  Local Theorem exec_equiv_congruence : forall T (p1 p2: proc Op T) T' (rx1 rx2: T -> proc Op T'),
+      exec_equiv_rx p1 p2 ->
+      (forall x, exec_equiv_rx (rx1 x) (rx2 x)) ->
+      exec_equiv_rx (Bind p1 rx1) (Bind p2 rx2).
+  Proof.
+    intros.
+    unfold exec_equiv_rx; intros.
+    repeat rewrite exec_equiv_bind_bind.
+    etransitivity.
+    eapply H.
+    eapply exec_equiv_bind_a; intros.
+    eapply H0.
+  Qed.
+
+  Theorem exec_equiv_rx_bind_a : forall `(p : proc Op T) `(p1 : T -> proc _ T') p2,
+      (forall x, exec_equiv_rx (p1 x) (p2 x)) ->
+      exec_equiv_rx (Bind p p1) (Bind p p2).
+  Proof.
+    intros.
+    eapply exec_equiv_rx_proof_helper; intros.
+    - exec_tid_inv.
+      exec_tid_inv.
+      ExecPrefix tid tid'.
+      destruct result; eauto.
+      eapply H; eauto.
+      apply exec_equiv_bind_bind.
+      apply exec_equiv_bind_bind in H3.
+      eapply exec_equiv_bind_a; intros; eauto; simpl.
+      symmetry.
+      eapply H; eauto.
+    - exec_tid_inv.
+      exec_tid_inv.
+      ExecPrefix tid tid'.
+      destruct result; eauto.
+      eapply H; eauto.
+      apply exec_equiv_bind_bind.
+      apply exec_equiv_bind_bind in H3.
+      eapply exec_equiv_bind_a; intros; eauto; simpl.
+      eapply H; eauto.
+  Qed.
+
+  Theorem exec_equiv_atomicret_ret : forall `(v : T),
+      exec_equiv_rx (Atomic (Ret v)) (Ret v).
+  Proof.
+    intros.
+    eapply exec_equiv_rx_proof_helper; intros; exec_tid_simpl.
+    - repeat atomic_exec_inv.
+      ExecPrefix tid tid'.
+    - ExecPrefix tid tid'.
+  Qed.
+
+  Theorem exec_equiv_until : forall `(p : option T -> proc Op T) (c : T -> bool) v,
+      exec_equiv_rx (Until c p v) (until1 c p v).
+  Proof.
+    intros.
+    eapply exec_equiv_rx_proof_helper; intros.
+    - exec_tid_simpl.
+      rewrite thread_upd_same_eq with (tid:=tid') in H2 by congruence.
+      simpl; eauto.
+    - abstract_tr.
+      ExecPrefix tid tid'.
+      ExecPrefix tid tid'.
+      rewrite <- prepend_app; auto.
+  Qed.
+
+  Theorem exec_equiv_spawn : forall `(p1 : proc Op T) p2,
+      exec_equiv p1 p2 ->
+      exec_equiv_rx (Spawn p1) (Spawn p2).
+  Proof.
+    intros.
+    eapply exec_equiv_rx_proof_helper; intros.
+    - exec_tid_simpl.
+      ExecPrefix tid tid'.
+      rewrite thread_upd_ne_comm in * by auto.
+      match goal with
+      | H : exec_equiv _ _ |- _ =>
+        apply H; eauto
+      end.
+    - exec_tid_simpl.
+      ExecPrefix tid tid'.
+      rewrite thread_upd_ne_comm in * by auto.
+      match goal with
+      | H : exec_equiv _ _ |- _ =>
+        apply H; eauto
+      end.
+  Qed.
+
+  Global Instance Bind_exec_equiv_proper :
+    Proper (exec_equiv_rx ==>
+                          pointwise_relation T exec_equiv_rx ==>
+                          @exec_equiv_rx TR) Bind.
+  Proof.
+    unfold Proper, respectful, pointwise_relation; intros.
+    apply exec_equiv_congruence; auto.
+  Qed.
+
+  Global Instance Spawn_exec_equiv_proper :
+    Proper (@exec_equiv T ==> exec_equiv_rx) Spawn.
+  Proof.
+    unfold Proper, respectful, pointwise_relation; intros.
+    apply exec_equiv_spawn; auto.
+  Qed.
+
+  Global Instance exec_proper_exec_equiv :
+    Proper (eq ==> exec_equiv_ts ==> eq ==> iff) (@exec Op State op_step).
+  Proof.
+    unfold Proper, respectful; intros; subst; eauto.
+  Qed.
+
+  Global Instance SpawnN_exec_equiv_proper :
+      Proper (eq ==> (exec_equiv (T:=T)) ==> exec_equiv_rx) SpawnN.
+  Proof.
+    unfold Proper, respectful; intros; subst.
+    induction y; simpl.
+    - reflexivity.
+    - rewrite H0.
+      setoid_rewrite IHy.
+      reflexivity.
+  Qed.
+
+End OpSemantics.
